\section*{Problem 3}

Find the output for the system in null state:

\begin{equation*}
\begin{aligned}
y[n] = \frac{1}{2} y[n-1] + 4x[n] + 3x[n-1]
\end{aligned}
\end{equation*} 

To the input:
\begin{equation*}
\begin{aligned}
x[n]=e^{j n \pi/3} u[n]
\end{aligned}
\end{equation*} 

\subsection*{Solution}
Since the system is at null state we have:
\begin{equation*}
\begin{aligned}
y[-1] &= 0\\
x[-1] &= 0
\end{aligned}
\end{equation*} 

The Z-Transform of the input $x[n]$ is:
\begin{equation*}
\begin{aligned}
x[z] = \frac{z}{z-e^{j\pi/3}}
\end{aligned}
\end{equation*} 

Therefore,

\begin{equation*}
\begin{aligned}
y[z] &= \frac{1}{2} z^{-1}y[z] + 4x[z] + 3z^{-1}x[z] \\
\frac{y[z]}{z} &= \frac{x[z]z^{-1}(4z+3)}{z-\frac{1}{2}}) \\
&= \frac{4z+3}{z-0.5)z} \frac{z}{z-e^{j\pi/3}}\\
&= \frac{A}{z-0.5} + \frac{B}{z-e^{j\pi/3}}
\end{aligned}
\end{equation*} 

From partial fractions we have:
\begin{equation*}
\begin{aligned}
A &= \frac{5}{0.5-e^{j\pi/3}} = 5.77j \\
B &= \frac{4e^{j\pi/3}+3}{e^{j\pi/3}-0.5} = 4-5.77j
\end{aligned}
\end{equation*}

Therefore,

\begin{equation*}
\begin{aligned}
y[z] &= A \frac{z}{z-0.5} + B \frac{z}{z-e^{j\pi/3}} \\
y[n] &= A (0.5)^n + B (e^{j\pi/3})^n\\
&= 5.77j (0.5)^n + (4-5.77j)e^{jn\pi/3}
\end{aligned}
\end{equation*} 
